hax-lib/core-models/README.md
@@ -3,3 +3,9 @@ This crate contains a partial model of Rust core that should preserve the same t
 ## Contributing
 
 Currently the only backend supported is F*, and the extracted models coexist with hand-written F* models. When a new module is added, the hand-written version should be deleted and replaced by the generated one. `.hax.sh extract` takes care of extracting and placing the result in `proof-libs`.
+
+## Style considerations
+
+Here is a list of things to pay attention to when contributing to the models:
+* When using the `Fn` traits, the syntax shortcuts `Fn(T) -> U` are not available for the model traits. We need to write `Fn<T, Output = U>`
+* The `core.mem.take` function cannot be given a good model that fits the Rust interface, we can only make it use unsafe or the original version, or change the interface to something corresponding to the interface of translated code (state passing instead of `&mut`).
